admitted equiv proof

src/Gc.v
@@ -63,74 +63,18 @@ Proof.
     crush.
 Qed.
 
-Lemma set_diff_union :
-  forall {A: Type} (eq_dec : forall (x y: A), {x = y} + {x <> y})
-         a b c,
-    length (set_diff eq_dec (set_union eq_dec a b) (set_union eq_dec a c)) =
-    length (set_diff eq_dec b c).
-Proof.
-Admitted.
-
-Lemma set_diff_union_rewrite :
-  forall {A: Type} (eq_dec : forall (x y: A), {x = y} + {x <> y})
-         a b c foo,
-  length (set_diff eq_dec (set_union eq_dec a b) (set_union eq_dec a c)) = foo ->
-  length (set_diff eq_dec b c) = foo.
-Proof.
-  intros.
-  specialize (set_diff_union eq_dec a b c).
-  crush.
-Qed.
-
-Lemma set_diff_union_rewrite_inv :
-  forall {A: Type} (eq_dec : forall (x y: A), {x = y} + {x <> y})
-         a b c foo,
-    length (set_diff eq_dec b c) = foo ->
-    length (set_diff eq_dec (set_union eq_dec a b) (set_union eq_dec a c)) = foo.
-Proof.
-  intros.
-  specialize (set_diff_union eq_dec a b c).
-  crush.
-Qed.
-
-  (*
-  induction a ; intros.
-  * admit.
-  * specialize IHa with b c.
-    unfold set_union in *. fold set_union in *.
-  * crush.
-  * crush.
-  * specialize IHb with nil.
-    assert ((set_union eq_dec nil nil) = nil). crush.
-    rewrite H in *. clear H.
-
-    assert ((length (set_diff eq_dec (a :: b) nil)) = length (a::b)).
-    unfold set_diff. destruct (set_mem eq_dec a nil) eqn:?. crush. crush.
-
-    unfold set_union. fold set_union.
-    unfold set_diff. fold set_diff.
-    destruct (set_mem eq_dec a nil) eqn:?. crush.
-    unfold set_add. fold set_add.
-  * admit.
-  * admit.
-  * admit.
-  * admit.
-  * admit.
-Qed.
- *)
-
 Fixpoint mark_ptr (fuel:nat) (p: ptr) (h: heap_t) : set ptr :=
   match fuel, heap_get_struct p h with
   | S n, Some vs =>
-      (set_union ptr_eq_dec (set_add ptr_eq_dec p (empty_set ptr))
+    (set_add ptr_eq_dec p
         (union_pointers
-          (List.map
-            (fun v =>
-              match v with
-              | Int _ => nil
-              | Pointer p' => mark_ptr n p' h
-              end
-           ) vs)))
+           (List.map
+              (fun v =>
+                 match v with
+                 | Int _ => nil
+                 | Pointer p' => mark_ptr n p' h
+                 end
+              ) vs)))
   | _, _ => nil
   end
 .
@@ -142,7 +86,7 @@ Theorem mark_ptr_subset:
 Proof.
   induction f ; crush.
   destruct (heap_get_struct p h) eqn:?.
-  specialize (set_union_elim _ _ _ _ H). intros.
+  specialize (set_add_elim _ _ _ _ H). intros.
   destruct H0.
   * exists l. unfold heap_get_struct.
     clear IHf H.
@@ -181,10 +125,9 @@ Proof.
   unfold mark_ptr.
   fold mark_ptr.
   destruct (heap_get_struct p h). Focus 2. crush.
-  specialize (set_union_elim _ _ _ _ H). intros. destruct H0.
-  inversion H0. eapply set_union_intro1. crush.
-  inversion H1.
-  eapply set_union_intro2.
+  specialize (set_add_elim _ _ _ _ H). intros. destruct H0.
+  subst. eapply set_add_intro2. reflexivity.
+  eapply set_add_intro1.
 
   specialize (nth_union_pointers_inv _ _ H0). intros. destruct H1. clear H0.
   eapply (nth_union_pointers _ x).
@@ -198,7 +141,7 @@ Proof.
            | Pointer p' =>
                match heap_get_struct p' h with
                | Some vs =>
-                   set_union ptr_eq_dec (set_add ptr_eq_dec p' (empty_set ptr))
+                   set_add ptr_eq_dec p'
                      (union_pointers
                         (map
                            (fun v0 : val =>
@@ -246,418 +189,25 @@ Proof.
       eapply mark_ptr_monotonic_1.
       auto.
 Qed.
-Theorem mark_ptr_saturates_1 :
-  forall f p h,
-    length (set_diff ptr_eq_dec (mark_ptr (S f) p h) (mark_ptr f p h)) = 0 ->
-    length (set_diff ptr_eq_dec (mark_ptr (S (S f)) p h) (mark_ptr (S f) p h)) = 0.
+
+Theorem mark_ptr_monotonic_3 :
+  forall f p h vs,
+    heap_maps_struct h p vs ->
+    set_In p (mark_ptr (S f) p h).
 Proof.
-  Admit.
-
-
-
-  induction f.
-  * admit.
-  * intros.
-    unfold mark_ptr in H ; fold mark_ptr in H.
-    unfold mark_ptr ; fold mark_ptr.
-    destruct (heap_get_struct p h). Focus 2. crush.
-    specialize (set_diff_union_rewrite _ _ _ _ _ H). clear H. intros.
-    eapply set_diff_union_rewrite_inv.
-    induction l.
-    - crush.
-    -
-      eapply IHf.
-
-
-
-    specialize (set_diff_union_rewrite _ _ _ _ _ H). clear H. intros.
-    specialize (set_diff_union ptr_eq_dec
-                               (set_add ptr_eq_dec p (empty_set ptr)) (union_pointers
-                 (map
-                    (fun v : val =>
-                     match v with
-                     | Int _ => nil
-                     | Pointer p' =>
-                         match heap_get_struct p' h with
-                         | Some vs =>
-                             set_union ptr_eq_dec
-                               (set_add ptr_eq_dec p' (empty_set ptr))
-                               (union_pointers
-                                  (map
-                                     (fun v0 : val =>
-                                      match v0 with
-                                      | Int _ => nil
-                                      | Pointer p'0 => mark_ptr f p'0 h
-                                      end) vs))
-                         | None => nil
-                         end
-                     end) l)) (union_pointers
-                 (map
-                    (fun v : val =>
-                     match v with
-                     | Int _ => nil
-                     | Pointer p' => mark_ptr f p' h
-                     end) l))).
-    unfold ptr in *.
-    unfold set in *.
-    intros.
-    rewrite H0 in H.
-    clear H0.
-    eapply set_diff_union.
-
-Admitted.
-
-Theorem mark_ptr_saturates_1 :
-  forall f p h,
-    length (mark_ptr (S f) p h) = length (mark_ptr f p h) ->
-    length (mark_ptr (S (S f)) p h) = length (mark_ptr f p h).
-Proof.
-  induction f.
-  * crush.
-    destruct (heap_get_struct p h).
-    - admit.
-    - auto.
-  * intros.
-
+  intros.
+  crush.
+  eapply set_add_intro2.
+  crush.
 Qed.
 
-
-Theorem mark_ptr_saturates_1 :
-  forall h e p,
-  exists f,
-    set_In e (mark_ptr (S f) p h) ->
-    set_In e (mark_ptr f p h).
-Proof.
-Admitted.
-
-(* each addition fuel gives it at least one, up until it saturates *)
-(* highest anything can saturate is length *)
-
-Theorem mark_ptr_saturates_1 :
+Theorem mark_ptr_saturates :
   forall h e p,
     set_In e (mark_ptr (S (length h)) p h) ->
     set_In e (mark_ptr (length h) p h).
 Proof.
-  intros.
-
-  destruct (set_In_dec ptr_eq_dec e (mark_ptr (length h) p h)). auto.
-  contradict n.
-  intros.
-  remember (length h) as n.
-  revert Heqn H.
-  induction n.
-  * crush. admit.
-  * intros.
-  unfold mark_ptr in H ; fold mark_ptr in H.
-  assert (exists n, (length h = S n)). destruct h. crush. exists (length h). crush.
-
-  destruct H0.
-
-  induction x.
-  * rewrite H0. unfold mark_ptr ; fold mark_ptr.
-    destruct (heap_get_struct p h) eqn:?. Focus 2. crush.
-    destruct (ptr_eq_dec p e) eqn:?.
-    - eapply set_union_intro1. crush.
-    - eapply set_union_intro2.
-      specialize (set_union_elim _ _ _ _ H). intros. destruct H1.
-      + inversion H1. Focus 2. crush. crush.
-      + clear H.
-
-        specialize (nth_union_pointers_inv _ _ H1). intros. destruct H. clear H1.
-        specialize (@map_nth
-                      val
-                      (list ptr)
-                      (fun v : val =>
-                         match v return list ptr with
-                         | Int _ => nil
-                         | Pointer p' => mark_ptr (length h) p' h
-                         end) l (Int 0) x).
-        unfold ptr. unfold set.
-        unfold ptr in H. unfold set in H.
-        intros.
-        rewrite H1 in H.
-        clear H1.
-        eapply (nth_union_pointers _ x).
-        specialize (@map_nth
-                      val
-                      (list ptr)
-                      (fun v : val =>
-                         match v return list ptr with
-                         | Int _ => nil
-                         | Pointer p' => nil
-                         end) l (Int 0) x).
-        unfold ptr. unfold set.
-        intros.
-        rewrite H1.
-        clear H1.
-        destruct (nth x l (Int 0)). crush.
-        unfold ptr in H. unfold ptr in H0.
-        rewrite H0 in H.
-        unfold mark_ptr in H.
-        admit.
-  *
-
-        specialize (
-
-        rewrite H0 in H1. unfold mark_ptr in H1 ; fold mark_ptr in H1.
-
-        subst.
-        eapply set_union_intro1. crush.
-    - eapply set_union_intro2. clear H.
-
-
-  rewrite H0. unfold mark_ptr ; fold mark_ptr.
-  destruct (heap_get_struct p h) eqn:?. Focus 2. crush.
-  specialize (set_union_elim _ _ _ _ H). intros. destruct H1.
-  * inversion H1. Focus 2. crush.
-    subst.
-    eapply set_union_intro1. crush.
-  * eapply set_union_intro2. clear H.
-
-
- edestruct (heap_get_struct p h) eqn:?. unfold heap_get_
-
-  destruct (set_In_dec ptr_eq_dec e (mark_ptr (length h) p h)). auto.
-  specialize (mark_ptr_monotonic_3 (length h) e p h H n).
-  intros.
-  destruct H0. destruct H0. destruct H0.
-
-  induction h. crush.
-  intuition.
-
-
-  induction h.
-  * intros. crush.
-  * intros.
-    assert (length (a::h) = S (length h)). crush. rewrite H0. clear H0.
-    unfold mark_ptr ; fold mark_ptr.
-
-
-
-  pose (0:nat).
-  intros h.
-  assert (length h = length h - n). crush.
-  rewrite H.
-  induction n.
-  * intros.
-    rewrite H.
-
-  intros h.
-  pose ((length h):nat).
-  assert (n = length h). crush.
-  rewrite <- H.
-  assert (n >= length h). crush. clear H.
-  induction n. assert (length h = 0). inversion H0. crush. assert (h = nil). eapply length_zero_iff_nil. crush. crush.
-  intros.
-  destruct (PeanoNat.Nat.eq_dec n (length h)).
-  * subst.
-    assert (length h >= length h). crush.
-    intuition. clear H1.
-    specialize (H2 e p).
-  *
-
-  induction (length h) eqn:? ; intros. assert (h = nil). eapply length_zero_iff_nil. crush. crush.
-
-  crush.
-
-  destruct h. crush.
-  assert (length (p0::h) = S (length h)). crush. rewrite H1. clear H1.
-  destruct p0.
-
-  unfold mark_ptr in H ; fold mark_ptr in H.
-  unfold mark_ptr ; fold mark_ptr.
-  destruct (heap_get_struct p ((p0, l) :: h)).
-  * specialize (set_union_elim _ _ _ _ H). intros. destruct H1.
-    - eapply set_union_intro1. crush.
-    - eapply set_union_intro2.
-      clear H.
-      specialize (nth_union_pointers_inv _ _ H1). intros. destruct H. clear H1.
-      eapply (nth_union_pointers _ x).
-
-      specialize (@map_nth
-                    val
-                    (list ptr)
-                    (fun v : val =>
-                       match v return list ptr with
-                       | Int _ => nil
-                       | Pointer p' => mark_ptr (length h) p' ((p0,l)::h)
-                       end) l0 (Int 0) x).
-      intros. rewrite H1. clear H1.
-
-      specialize (@map_nth
-                    val
-                    (list ptr)
-                    (fun v : val =>
-                       match v return list ptr with
-                       | Int _ => nil
-                       | Pointer p' => mark_ptr f p' ((p0,l)::h)
-                       end) l0 (Int 0) x).
-      intros.
-      unfold ptr in H; unfold ptr in H1 ; unfold set in H ; unfold set in H1.
-      rewrite H1 in H. clear H1.
-      destruct (nth x l0 (Int 0)). crush.
-      specialize (IHf ((p0,l)::h) e p1). intuition.
-      destruct (Compare_dec.le_gt_dec f (length ((p0,l) :: h))).
-      + assert (f = length ((p0, l) :: h)). crush.
-        subst. clear H0 l1 H1.
 Admitted.
-(*
-        eapply mark_ptr_saturates_1.
-      + intuition.
-      eapply IHf.
-  * crush.
-Qed.
-  intros.
-  assert (exists n, length h = S n). destruct h. crush. exists (length h). crush.
-  destruct H1.
-  specialize (IHf h e).
-  rewrite H1 in *. clear H1.
-  clear IHf.
-  induction x ; induction f ; try solve [crush].
-  *
-  rewrite H1.
-  destruct (Compare_dec.gt_dec f (S x)). Focus 2. assert (f = S x). crush. subst. clear n. clear H0. rewrite <- H1 in *. clear H1. clear IHf.
-  admit.
-  specialize (IHf p).
-  eapply IHf.
 
-  * admit.
-  *
-  unfold mark_ptr in *. fold mark_ptr in *.
-  specialize (IHf h e p).
-
-  induction h. intros. assert (exists f', f = S f'). inversion H0. crush. crush. crush.
-  intros.
-  assert (length (a::h) = S (length h)). crush. rewrite H1. clear H1.
-
-  induction f. crush.
-  intros.
-
-
-  intros.
-  eapply IHf.
-
-  destruct h. crush.
-  intros.
-
-  assert (length (a::h) = S (length h)). crush. rewrite H1. clear H1.
-  unfold mark_ptr in * ; fold mark_ptr in *.
-
-  unfold mark_ptr.
-Qed.
-
-Theorem mark_ptr_saturates :
-  forall f h e p,
-    set_In e (mark_ptr f p h) ->
-    set_In e (mark_ptr (length h) p h).
-Proof.
-  induciton f
-
-
-  induction f ; induction h ; try solve [crush].
-  intros.
-  assert (length (a::h) = S (length h)). crush. rewrite H0. clear H0.
-  unfold mark_ptr in * ; fold mark_ptr in *.
-  destruct a.
-  destruct (ptr_eq_dec p0 p) eqn:?.
-  * unfold heap_get_struct in *. rewrite Heqs in *.
-    destruct (ptr_eq_dec e p) eqn:?.
-    - eapply set_union_intro1. crush.
-    - eapply set_union_intro2.
-      specialize (set_union_elim ptr_eq_dec _ _ _ H).
-      intros.
-      destruct H0 ; crush.
-      specialize (nth_union_pointers_inv _ _ H0).
-      intros. destruct H1.
-      eapply (nth_union_pointers _ x).
-      specialize (@map_nth
-                    val
-                    (list ptr)
-                    (fun v : val =>
-                       match v return list ptr with
-                       | Int _ => nil
-                       | Pointer p' => mark_ptr (length h) p' ((p,l)::h)
-                     end) l (Int 0) x).
-      intros. rewrite H2 ; clear H2.
-
-      specialize (@map_nth
-                    val
-                    (set ptr)
-                    (fun v : val =>
-                       match v with
-                       | Int _ => nil
-                       | Pointer p' => mark_ptr f p' ((p, l) :: h)
-                       end) l (Int 0) x).
-      intros. intuition.
-      unfold set in H1.
-      unfold set in H2.
-      unfold ptr in H2.
-      unfold ptr in H1.
-      rewrite H2 in H1. clear H2.
-      specialize (nth_default_eq x l (Int 0)). intros.
-      rewrite <- H2. rewrite <- H2 in H1. intros. clear H2.
-      destruct (nth_default (Int 0) l x) eqn:?. crush.
-
-      specialize (nth_default_eq x l (Int 0)). intros.
-      unfold n
-
-      specialize (@nth_default_eq (set ptr) x (map
-               (fun v : val =>
-                match v with
-                | Int _ => nil
-                | Pointer p' => mark_ptr f p' ((p, l) :: h)
-                end) l) (@nil nat)).
-      intros.
-      rewrite <- H2 in H1.
-      clear H2.
-
-      destruct ((@nth_default (set ptr) (@nil nat)
-            (@map val (list ptr)
-               (fun v : val =>
-                match v return (list ptr) with
-                | Int _ => @nil ptr
-                | Pointer p' =>
-                    mark_ptr f p'
-                      (@cons (prod ptr (list val)) (@pair ptr (list val) p l) h)
-                end) l) x)). crush
-      destruct ((nth_default nil
-            (map
-               (fun v : val =>
-                match v with
-                | Int _ => nil
-                | Pointer p' => mark_ptr f p' ((p, l) :: h)
-                end) l) x)) eqn:?.
-      rewrite Heql0 in H1.
-
-      edestruct nth_default eqn:?. crush.
-
-      specialize (@map_nth
-                    val
-                    (list ptr)
-                    (fun v : val =>
-                       match v return list ptr with
-                       | Int _ => @nil ptr
-                       | Pointer p' => mark_ptr f p' ((p,l)::h)
-                       end) l (Int 0) x).
-      intros. intuition.
-      rewrite H2 in H1.
-
-      specialize (map_ne
-      unfold nth_default. rewrite H0.
-      specailze
-      eapply IHh.
-Admitted.
-(*
-  induction f ; induction h ; crush.
-  destruct (ptr_eq_dec a0 p) eqn:?.
-  *
-  * crush.
-  * induction h.
-  - crush.
-  - intros.
-Admitted.
-*)
-*)
 Theorem mark_ptr_marks :
   forall address h p p',
     addresses h p address p' ->
@@ -675,18 +225,17 @@ Proof.
       rewrite H0.
       unfold mark_ptr.
       rewrite H.
-      apply set_union_iff; crush.
+      apply set_add_iff; crush.
   * intros.
     inversion H.
     subst.
     specialize (IHaddress h p'0 p' H6).
-    assert (exists n0, set_In p' (mark_ptr n0 p h)).
-    - exists (S (length h)).
-      unfold mark_ptr ; fold mark_ptr.
+    assert (set_In p' (mark_ptr (S (length h)) p h)).
+    - unfold mark_ptr ; fold mark_ptr.
       specialize (heap_maps_implies_heap_get h p n (Pointer p'0) H4).
       intros. destruct H0. destruct H0.
       rewrite H0.
-      eapply set_union_intro2.
+      eapply set_add_intro1.
       eapply (nth_union_pointers _ n).
 
       specialize (@map_nth
@@ -702,8 +251,8 @@ Proof.
       rewrite <- H2. intros. clear H2.
       unfold nth_default. rewrite H1.
       auto.
-    - destruct H0.
-      eapply mark_ptr_saturates. apply H0.
+    - eapply mark_ptr_saturates.
+      apply H0.
 Qed.
 
 Theorem mark_ptr_correct :
@@ -727,7 +276,7 @@ Proof.
     clear Heqo.
     clear Heqe.
     clear e.
-    apply set_union_iff in H.
+    apply set_add_iff in H.
     destruct H.
     * crush.
       eauto.
@@ -751,7 +300,6 @@ Proof.
                  eapply (FollowAddresses h p p0 p'); subst; eauto.
            ** apply IHl; intuition.
 Qed.
-
 
 Fixpoint mark (r: roots_t) (h: heap_t) : set ptr :=
   match r with
@@ -777,10 +325,10 @@ Definition gc (r: roots_t) (h: heap_t) : heap_t :=
 .
 
 Theorem heap_marks :
-  forall address roots heap var ptr ptr',
-    roots_maps roots var ptr ->
-    addresses heap ptr address ptr' ->
-    set_In ptr' (mark roots heap)
+  forall address r h v p p',
+    roots_maps r v p ->
+    addresses h p address p' ->
+    set_In p' (mark r h)
 .
 Proof.
   Hint Resolve set_union_iff.
@@ -806,190 +354,193 @@ Proof.
         crush.
 Qed.
 
-
-Lemma pointer_equivalence :
-  forall address r h v p p' h',
-    roots_maps r v p ->
+Lemma address_extend :
+  forall address h p p' p'' n n' v,
     addresses h p address p' ->
-    sweep h (mark r h) = h' ->
-    addresses h' p address p'.
+    heap_maps h p' n (Pointer p'') ->
+    heap_maps h p'' n' v ->
+    (exists address', addresses h p address' p'').
 Proof.
-  induction address.
-  * intros.
-    specialize (heap_marks TermStr r h v p p' H H0).
-    intros.
-    inversion H0. subst.
+  induction address ; intros.
+  * inversion H. destruct H2. subst. clear H.
+    exists (FollowStr n TermStr).
+    eapply (FollowAddresses h p' p'' p'' n TermStr). auto.
     constructor.
-    destruct H3.
-    exists x.
-    induction h ; crush.
-    destruct a.
-    destruct (ptr_eq_dec p p'). subst.
-    - unfold heap_maps_struct in H1. unfold heap_get_struct in H1.
-      destruct (ptr_eq_dec p' p') ; crush.
-      assert (set_mem ptr_eq_dec p' (mark r ((p', x) :: h)) = true).
-      eapply set_mem_correct2. auto.
-      crush.
-      unfold heap_maps_struct. unfold heap_get_struct.
-      destruct (ptr_eq_dec p' p') ; crush.
-    - assert (set_mem ptr_eq_dec p (mark r ((p, l) :: h)) = true).
-      unfold mark.
-      induction r. crush.
-      destruct a.
-      destruct (ptr_eq_dec p0 p).
-      + subst.
-        eapply set_mem_correct2.
-        eapply set_union_intro2.
-        assert (length ((p, l) :: h) = S (length h)). crush.
-        rewrite H3. clear H3.
-        unfold mark_ptr. fold mark_ptr.
-        unfold heap_get_struct. fold heap_get_struct.
-        destruct (ptr_eq_dec p p) ; crush.
-        eapply set_union_intro1. crush.
-      + assert (roots_maps r v p'). unfold roots_maps in *. unfold In in H.
-        destruct H. injection H. intros. rewrite H3 in n0.
-        assert (addresses h p' TermStr p').
-
-
-    eapply TermAddresses.
-
-    constructor.
-    eapply heap_marks.
+    unfold heap_maps in H1. unfold heap_get in H1.
+    destruct (heap_get_struct p'' h) eqn:?. exists l. auto. crush.
+  * crush.
+    inversion H. clear H. subst.
+    specialize (IHaddress h p'0 p' p'' n0 n' v).
+    intuition.
+    destruct H.
+    exists (FollowStr n x).
+    eapply (FollowAddresses h p p'0 p'' n x) ; auto.
 Qed.
 
-(* Must be proved for liveness *)
-Lemma pointer_equivalence :
-  forall address s v p p' h,
-    roots_maps (roots s) v p ->
-    addresses (heap s) p address p' ->
-    sweep (heap s) (mark (roots s) (heap s)) = h ->
-    addresses h p address p'.
+Lemma pointer_equivalence' :
+  forall address r h p p',
+    addresses h p address p' ->
+    set_In p (mark r h) ->
+    addresses (sweep h (mark r h)) p address p'.
 Proof.
   induction address.
-  * intros.
-    inversion H0; subst.
-    destruct H2.
-    constructor.
-    exists x.
-    induction (heap s); crush.
+  * crush. inversion H. clear H. destruct H1.
+    crush.
+    remember (mark r h) as foo. clear Heqfoo.
+    induction h. inversion H.
     destruct a.
-    unfold heap_maps_struct in *.
+    unfold sweep in * ; fold sweep in *.
+    unfold heap_maps_struct in * ; fold heap_maps_struct in *.
+    unfold heap_get_struct in * ; fold heap_get_struct in *.
     destruct (ptr_eq_dec p p') eqn:?.
     - crush.
-      rewrite Heqs0 in H1.
-      edestruct set_mem eqn:?.
+      assert (set_mem ptr_eq_dec p' foo = true). eapply set_mem_correct2. auto.
+      rewrite H.
+      constructor. exists x. unfold heap_maps_struct. unfold heap_get_struct.
+      destruct (ptr_eq_dec p' p'). crush. crush.
+    - destruct (set_mem ptr_eq_dec p foo).
       + crush.
-      + contradict Heqb.
-        unfold mark.
-        crush.
-        clear - H2 H.
-        induction (roots s). crush.
-        destruct a.
-        destruct (ptr_eq_dec p p') eqn:?.
-        ** crush.
-           rewrite Heqs0 in H2.
-           specialize (set_mem_complete1 ptr_eq_dec p' _ H2).
-           intros. contradiction H0.
-           eapply set_union_intro2.
-           eapply set_union_intro1.
-           crush.
-        ** unfold roots_maps in *.
-           unfold In in H.
-           destruct H. crush.
-           intuition.
-           remember ((fix mark (r : roots_t) (h : heap_t) {struct r} :
-           set ptr :=
-             match r with
-             | nil => nil
-             | (_, ptr0) :: rest =>
-                 set_union ptr_eq_dec (mark rest h) (mark_ptr (length h) ptr0 h)
-             end) r ((p', x) :: h)) as foo.
-           clear - H0 H2.
-           assert (set_mem ptr_eq_dec p' foo = true).
-           destruct (set_In_dec ptr_eq_dec p' foo). eapply set_mem_correct2. auto.
-           specialize (set_mem_complete2 ptr_eq_dec p' foo n). auto.
-           specialize (set_mem_correct1 ptr_eq_dec p' foo H). intros.
-           specialize (set_mem_complete1 ptr_eq_dec p' _ H2). intros.
-           contradict H3.
-           eapply set_union_intro1. auto.
-    - assert (addresses h p' TermStr p').
-      constructor. unfold heap_maps_struct.
-      exists x.
-      crush.
-      rewrite Heqs0 in H1. crush.
-      intuition.
-      assert (heap_get_struct p' h = Some x). crush. rewrite Heqs0 in H1. crush.
-      intuition.
-      edestruct set_mem eqn:?.
-      + unfold heap_get_struct. rewrite Heqs0. fold heap_get_struct.
-        admit.
-      + admit.
-
-      edestruct set_mem eqn:?.
-
-           specialize (set_mem_complete1 ptr_eq_dec p' _ H0).
-           unfold not.
+        inversion H1. destruct H2. subst.
+        constructor. exists x0.
+        unfold heap_maps_struct. unfold heap_get_struct.
+        destruct (ptr_eq_dec p p'). crush. crush.
+      + crush.
+  * crush.
+    inversion H. clear H. subst.
+    specialize (IHaddress r h p'0 p' H7).
+    assert (set_In p'0 (mark r h)).
+    - clear IHaddress.
+      induction r. crush.
+      destruct a.
+      destruct (ptr_eq_dec p'0 p0) eqn:?.
+      + crush.
+        assert (exists x, length h = S x). destruct h. unfold heap_maps in H5. unfold heap_get in H5. crush. exists (length h). crush.
+        destruct H. rewrite H. unfold mark_ptr. fold mark_ptr.
+        clear H Heqs IHr H0 H5.
+        eapply set_union_intro2.
+        inversion H7.
+        ** destruct H. subst.
+           rewrite H. eapply set_add_intro2. auto.
+        ** subst.
+           unfold heap_maps in H. unfold heap_get in H.
+           destruct (heap_get_struct p0 h). Focus 2. crush.
+           eapply set_add_intro2. auto.
+      + unfold mark in * ; fold mark in *.
+        unfold set_In in *.
+        destruct (set_union_elim _ _ _ _ H0).
+        ** crush. eapply set_union_intro1. auto.
+        ** specialize (mark_ptr_correct _ _ _ _ H).
            intros.
-           assert (set_mem ptr_eq_dec p' foo = true).
-           unfo
-           crush.
-           contradict H1.
-           eapply set_union_intro1.
-           contradict H0.
-           crush.
-           unfold not in H1.
-           eapply H0 in H1.
-
-        unfold not. intros.
-        specialize (set_mem_complete1 ptr_eq_dec p' (set_union ptr_eq_dec
-            ((fix mark (r : roots_t) (h : heap_t) {struct r} :
-              set ptr :=
-                match r with
-                | nil => nil
-                | (_, ptr0) :: rest =>
-                    set_union ptr_eq_dec (mark rest h) (mark_ptr (length h) ptr0 h)
-                end) r ((p', l) :: h))
-            (mark_ptr (length ((p', l) :: h)) p ((p', l) :: h))) H2).
-        intros.
-        contradiction H3.
-
-        unfold mark_ptr.
-        assert ((length ((p', l) :: h)) = S (length h)). crush.
-        rewrite H4.
-        unfold hea
-
-
-      edestruct set_mem.
-    - unfold heap_maps_struct in *.
-      crush.
-      edestruct ptr_eq_dec. crush.
-      intuition.
-    unfold sweep.
-
-    eexists. apply H1.
-    crush.
-    inversion H2.
-    inversion H5.
-  * intros.
-    inversion H0.
-    subst.
-    remember (fuel s) as f.
-    induction f ; subst.
-  -  unfold gc, mark, sweep.
-
-      subst.
-      induction (fuel s).
-    -
-    induction v0.
-    - inversion H5.
-      subst.
-
-      inversion H5.
-      specialize (IHaddress s v p).
-    intuition.
-    eapply IHaddress.
- *)
+           destruct H1.
+           inversion H7.
+           -- subst. clear H7.
+              destruct H2.
+              specialize (set_union_elim _ _ _ _ H0). intros. clear H0.
+              destruct H3.
+              ++ intuition.
+                 eapply set_union_intro1. auto.
+              ++ eapply set_union_intro2. auto.
+                 destruct (ptr_eq_dec p' p). crush.
+                 assert (exists x, length h = S (S x)). destruct h. crush.
+                 admit.
+                 destruct H3. rewrite H3 in H0.
+                 destruct (heap_get_struct p0 h) eqn:?.
+                 *** unfold mark_ptr in H0. fold mark_ptr in H0.
+                     rewrite Heqo in H0.
+                     specialize (set_add_elim _ _ _ _ H0).
+                     intros. destruct H4 ; subst.
+                     --- rewrite H3.
+                         unfold mark_ptr in *. fold mark_ptr in *.
+                         rewrite Heqo.
+                         eapply set_add_intro1.
+                         eapply (nth_union_pointers _ n).
+                         unfold heap_maps in H5.
+                         unfold heap_get in H5.
+                         rewrite Heqo in H5.
+                         specialize (@map_nth
+                                       val
+                                       (list ptr)
+                                       (fun v : val =>
+           match v with
+           | Int _ => nil
+           | Pointer p'0 =>
+               match heap_get_struct p'0 h with
+               | Some vs =>
+                   set_add ptr_eq_dec p'0
+                     (union_pointers
+                        (map
+                           (fun v0 : val =>
+                            match v0 with
+                            | Int _ => nil
+                            | Pointer p'1 => mark_ptr x1 p'1 h
+                            end) vs))
+               | None => nil
+               end
+           end) l (Int 0) n).
+                         intros.
+                         unfold ptr in *. unfold set in *.
+                         rewrite H4. clear H4.
+                         specialize (nth_default_eq n l (Int 0)). intros.
+                         rewrite <- H4.
+                         unfold nth_default.
+                         rewrite H5.
+                         destruct x1.
+                         +++ unfold heap_maps_struct in H2.
+                             rewrite H2.
+                             eapply set_add_intro2. reflexivity.
+                         +++ crush.
+                             eapply set_add_intro2. reflexivity.
+                     --- clear H0.
+                         admit.
+                 *** inversion H1. crush. subst.
+                     unfold heap_maps in *. unfold heap_get in *.
+                     rewrite Heqo in H4. discriminate.
+           -- specialize (address_extend _ _ _ _ _ _ _ _ H1 H5 H2).
+              intros.
+              destruct H10.
+              eapply set_union_intro2.
+              eapply mark_ptr_marks.
+              apply H10.
+    - intuition.
+      eapply (FollowAddresses (sweep h (mark r h)) p p'0 p' n address).
+      + clear - H0 H5.
+        remember (mark r h) as foo. clear Heqfoo.
+        induction h. crush.
+        destruct a.
+        unfold sweep in * ; fold sweep in *.
+        unfold heap_maps in * ; fold heap_maps in *.
+        unfold heap_get in * ; fold heap_get in *.
+        unfold heap_get_struct in * ; fold heap_get_struct in *.
+        destruct (ptr_eq_dec p0 p) eqn:?.
+        ** crush.
+           assert (set_mem ptr_eq_dec p foo = true). eapply set_mem_correct2. auto.
+           rewrite H. crush.
+        ** crush.
+           destruct (set_mem ptr_eq_dec p0 foo).
+           -- crush.
+           -- crush.
+      + crush.
 Admitted.
+
+Lemma pointer_equivalence :
+  forall address r h v p p',
+    roots_maps r v p ->
+    addresses h p address p' ->
+    addresses (sweep h (mark r h)) p address p'.
+Proof.
+  intros.
+  eapply pointer_equivalence'.
+  apply H0.
+  eapply heap_marks.
+  apply H.
+  eapply TermAddresses.
+  inversion H0.
+  * apply H1.
+  * unfold heap_maps in H1. unfold heap_get in H1.
+    destruct (heap_get_struct p h) eqn:?.
+    - exists l. crush.
+    - crush.
+Qed.
 
 (*
 Theorem safety_1 :
